@prefix dc:   <http://purl.org/dc/terms/> .
@prefix ex:   <http://example.com#> .
@prefix foaf: <http://xmlns.com/foaf/0.1/> .
@prefix imf:  <http://ns.imfid.org/imf#> .
@prefix owl:  <http://www.w3.org/2002/07/owl#> .
@prefix pav:  <http://purl.org/pav/> .
@prefix rdf:  <http://www.w3.org/1999/02/22-rdf-syntax-ns#> .
@prefix rdfs: <http://www.w3.org/2000/01/rdf-schema#> .
@prefix sh:   <http://www.w3.org/ns/shacl#> .
@prefix skos: <http://www.w3.org/2004/02/skos/core#> .
@prefix vann: <http://purl.org/vocab/vann/> .
@prefix vs:   <http://www.w3.org/2003/06/sw-vocab-status/ns#> .
@prefix xsd:  <http://www.w3.org/2001/XMLSchema#> .

@prefix sym:  <http://example.equinor.com/symbol#> .

sym:SymbolOntology a owl:Ontology ;
    dc:title "Symbol Ontology" ;

    vann:preferredNamespacePrefix "sym" ;
    #TODO vann:preferredNamespaceUri
    #owl:priorVersion 
    #owl:versionIRI 
    owl:versionInfo "0.1.0-SNAPSHOT" ;
    # doap:repository

    dc:creator "Martin G. Skjæveland" ;
    dc:contributor "Arne Måge", "Lorentz Fjellanger Barstad" ;

    dc:created "2023-09-19" ;
    #dc:issued "2023-09-19"^^xsd:dateTime ;
    dc:modified "2023-09-26" ;

    dc:abstract "The Symbol Ontology is designed to be used for representing typically standardized engineering symbols that are used in technical drawings, diagrams, schematics, and blueprints, as well as for documentation and communication in engineering disciplines such as mechanical, electrical, civil, and chemical engineering." ;
    #dc:description "" ;
    #skos:changeNote    
.

sym:svg-path-data a rdfs:Datatype ;
  skos:definition "" ;
  rdfs:seeAlso "https://developer.mozilla.org/en-US/docs/Web/SVG/Tutorial/Paths" ;
.

sym:Symbol a owl:Class , sh:NodeShape , rdfs:Class ;
  skos:prefLabel "Symbol" ;
  skos:definition "A symbol is a graphical representation of an entity. A symbol has exactly one shape, which can be represented in multiple ways." ;
  # skos:changeNote
#  skos:example """
#nil  
#  """ ;
  sh:order 1;
  sh:property

    # RDFS
    [ sh:path rdfs:label ; sh:minCount 0; sh:nodeKind sh:Literal ;
        sh:name "Label" ; sh:order 1.1 ;
        sh:description "Human readable label of the symbol."] ,

    # DC
    [ sh:path dc:identifier ; sh:minCount 1 ; sh:maxCount 1 ; sh:nodeKind sh:IRIOrLiteral ;
        sh:name "Identifier" ; sh:order 1.2 ;
        sh:description "Identifier for the symbol that is stable over different versions of the symbol." ] ,

    [ sh:path dc:description ; sh:minCount 1 ; sh:nodeKind sh:Literal ; sh:severity sh:Warning ;
        sh:name "Description" ; sh:order 2.1 ;
        sh:description "Human readable description of the symbol." ] ,

    [ sh:path dc:source ; sh:minCount 0 ;
        sh:name "Source" ; sh:order 3.2 ;
        sh:description "Reference to the source of the symbol, if the symbol is taken from a diagram standard that can be referenced." ] ,

    [ sh:path dc:subject ; sh:minCount 0 ;
        sh:name "Subject" ; sh:order 3.1 ;
        sh:description "Reference to the origin of the symbol, if the origin symbol can be referenced." ] ,

    [ sh:path dc:created ; sh:minCount 1 ; sh:maxCount 1 ; sh:datatype xsd:dateTime ;
        sh:name "Created date" ; sh:order 4.1 ;
        sh:description "Timestamp for creation of symbol." ] ,

    [ sh:path dc:modified ; sh:minCount 0 ; sh:datatype xsd:dateTime ;
        sh:name "Modified date" ; sh:order 4.2 ;
        sh:description "Timestamp for modification of symbol. Multiple values permitted." ] ,

    [ sh:path dc:issued ; sh:maxCount 1 ; sh:datatype xsd:dateTime ;
        sh:name "Issued date" ; sh:order 4.3 ;
        sh:description "Timestamp for when the symbol is officially issued, i.e., its release timestamp." ] ,

    [ sh:path dc:creator ; sh:minCount 0 ; sh:nodeKind sh:BlankNodeOrIRI ;
        sh:name "Creator" ; sh:order 5.1 ;
        sh:description "Creator(s) of the symbol." ] ,

    [ sh:path dc:contributor ; sh:minCount 0 ; sh:nodeKind sh:BlankNodeOrIRI ;
        sh:name "Contributor" ; sh:order 5.2 ;
        sh:description "Contributor(s) to the creation or modification of the symbol." ] ,

    # PAV
    [ sh:path pav:version ; sh:minCount 1 ; sh:maxCount 1 ; sh:nodeKind sh:Literal ; sh:severity sh:Warning ;
        sh:name "Version" ; sh:order 2.2 ;
        sh:description "Version number indicating the version of the symbol." ] ,

    [ sh:path pav:previousVersion ; sh:nodeKind sh:IRI ; 
        sh:name "Previous version" ; sh:order 2.3 ;
        sh:description "Reference to a previous version of the symbol." ] ,
   
    # SYM, these get their name and description from the ontology spec.
    [ sh:path sym:hasShape ; sh:minCount 1 ; sh:maxCount 1 ; sh:node sym:Shape ; sh:order 6.1 ] ,
    [ sh:path sym:height ; sh:minCount 1 ; sh:maxCount 1 ; sh:datatype xsd:integer ; sh:order 6.2 ] ,
    [ sh:path sym:width ; sh:minCount 1 ; sh:maxCount 1 ; sh:datatype xsd:integer ; sh:order 6.3 ] ,
    [ sh:path sym:drawColor ; sh:maxCount 1 ; sh:order 6.4 ] ,
    [ sh:path sym:fillColor ; sh:maxCount 1 ; sh:order 6.5 ] ,
    [ sh:path sym:hasConnectionPoint ; sh:minCount 0 ; sh:node sym:ConnectionPoint ; sh:order 6.6 ;
      sh:description "The symbol's connection points." ]
.


sym:Point a owl:Class ;
  skos:prefLabel "Point" ;
  skos:definition "A point is a position in a coordinate system. A point has no extension." ;
  # skos:changeNote
.

sym:ConnectionPoint a owl:Class , sh:NodeShape , rdfs:Class ;
  sh:targetObjectsOf sym:hasConnectionPoint ;
  rdfs:subClassOf sym:Point ;
  skos:prefLabel "Connection Point" ;
  skos:definition "A connection point is a point that acts as a point of connection for edges and arrows pointing to/from the point." ;
  sh:order 3;
  # skos:changeNote

  sh:property
    [ sh:path dc:identifier ; sh:minCount 1 ; sh:maxCount 1 ; sh:nodeKind sh:IRIOrLiteral ;
      sh:name "Identifier" ; sh:order 1.1 ;
      sh:description "Unique identifier for connection points in the context of a symbol." ] ,

    [ sh:path sym:connectorDirection ; sh:minCount 1 ; sh:datatype xsd:integer ; sh:order 2.3  ] ,
    [ sh:path sym:positionX ; sh:minCount 1 ; sh:maxCount 1 ; sh:datatype xsd:integer ; sh:order 2.1 ] ,
    [ sh:path sym:positionY ; sh:minCount 1 ; sh:maxCount 1 ; sh:datatype xsd:integer ; sh:order 2.2  ] ,
    [ sh:path [ sh:inversePath sym:hasConnectionPoint ] ; sh:minCount 1 ; sh:maxCount 1 ; sh:node sym:Symbol ;
      sh:description "The symbol to which the connction point belongs." ; sh:order 1.2 ] 
.


sym:Shape a owl:Class , sh:NodeShape , rdfs:Class ;
  skos:prefLabel "Shape" ;
  skos:definition "A shape is a description of a graphical form. A symbol has exactly one shape, but the shape can have multiple serialisations." ;
  sh:order 2;
  # skos:changeNote

  sh:targetObjectsOf sym:hasShape ;
  sh:property
    [ sh:path sym:hasSerialization ; sh:minCount 0; sh:nodeKind sh:Literal ; sh:order 1.1 ;
      sh:name "Serialization" ; 
      sh:description "A (textual) serialization of the symbol." ] ,
    [ sh:path foaf:depiction ; sh:minCount 0; sh:nodeKind sh:IRI ; sh:order 1.2 ;
      sh:name "Depiction" ; 
      sh:description "An depiction or image of the symbol." ] 

.

sym:hasConnectionPoint a owl:ObjectProperty ;
  skos:prefLabel "has connection point" ;
  rdfs:domain sym:Symbol ;
  rdfs:range sym:ConnectionPoint .

sym:isConnectionPointOn a owl:ObjectProperty ;
  owl:inverseOf sym:hasConnectionPoint ;
  rdfs:subPropertyOf sym:isPointOn .

sym:isPointOn a owl:ObjectProperty , owl:FunctionalProperty ;
  rdfs:domain sym:Point ;
  rdfs:range sym:Symbol .
  
sym:hasShape a owl:ObjectProperty ;
  skos:prefLabel "has shape" ;
  rdfs:domain sym:Symbol ;
  rdfs:range sym:Shape .

sym:hasSerialization a owl:DatatypeProperty ;
  skos:prefLabel "has serialization" ;
  rdfs:domain sym:Shape .

sym:fillColor a owl:DatatypeProperty ;
  skos:prefLabel "Fill color" ;
  skos:definition "A suggested color for filling the area contained by the shape of a symbol." ;
  rdfs:domain sym:Symbol .

sym:drawColor a owl:DatatypeProperty ;
  skos:prefLabel "Draw color" ;
  skos:definition  "A suggested color for drawing the shape of a symbol." ;
  rdfs:domain sym:Symbol .

sym:connectorDirection a owl:DatatypeProperty ;
  skos:prefLabel "Connector Direction" ;
  skos:definition "In degrees (usually in the range 0--359, and typically a factor of 90) the direction an inwards or outwards connector or edge can be connected to a connection point." ; 
  rdfs:domain sym:ConnectionPoint ;
  rdfs:range xsd:integer .

sym:positionX a owl:DatatypeProperty ;
  skos:prefLabel "X position" ;
  skos:definition "The X position of the connection point in px units relative to its symbol's (0,0) point." ;
  rdfs:domain sym:Point ;
  rdfs:range xsd:integer ;
  rdfs:seeAlso <https://developer.mozilla.org/en-US/docs/Web/SVG/Tutorial/Positions#what_are_pixels> .

sym:positionY a owl:DatatypeProperty ;
  skos:prefLabel "Y position" ;
  skos:definition "The Y position of the connection point in px units relative to its symbol's (0,0) point." ;
  rdfs:domain sym:Point ;
  rdfs:range xsd:integer .

sym:height a owl:DatatypeProperty ;
  skos:prefLabel "Height" ;
  skos:definition "The height of the symbol in px units." ;
  rdfs:domain sym:Symbol ;
  rdfs:range xsd:integer .

sym:width a owl:DatatypeProperty ;
  skos:prefLabel "Width" ;
  skos:definition "The width of the symbol in px units." ;
  rdfs:domain sym:Symbol ;
  rdfs:range xsd:integer .

sym:SymbolVocabularyShape a sh:NodeShape ;
    sh:message "Unrecognised Symbol vocabulary element. Check spelling." ;
    sh:name "Symbol vocabulary element." ;
    rdfs:comment "This shape ensures that the namespace of the Symbol ontology is only used for terms that are defined in the ontology. This helps avoid introducing undefined terms and typos." ;
    sh:sparql [ a sh:SPARQLConstraint ;
            sh:select """
	      SELECT DISTINCT ?value 
	      WHERE { { ?value ?p ?o }
	        UNION { ?s ?value ?o }
	        UNION { ?s ?p ?value }
	      FILTER (isIRI(?value) 
	        && STRSTARTS(STR(?value), 'http://example.equinor.com/symbol#'))
	      FILTER (?value NOT IN (
<http://example.equinor.com/symbol#ConnectionPoint>,
<http://example.equinor.com/symbol#Point>,
<http://example.equinor.com/symbol#Shape>,
<http://example.equinor.com/symbol#Symbol>,
<http://example.equinor.com/symbol#SymbolOntology>,
<http://example.equinor.com/symbol#connectorDirection>,
<http://example.equinor.com/symbol#drawColor>,
<http://example.equinor.com/symbol#fillColor>,
<http://example.equinor.com/symbol#hasConnectionPoint>,
<http://example.equinor.com/symbol#hasSerialization>,
<http://example.equinor.com/symbol#hasShape>,
<http://example.equinor.com/symbol#isConnectionPointOn>,
<http://example.equinor.com/symbol#isPointOn>,
<http://example.equinor.com/symbol#positionX>,
<http://example.equinor.com/symbol#positionY>,
<http://example.equinor.com/symbol#height>,
<http://example.equinor.com/symbol#width>,
<http://example.equinor.com/symbol#svg-path-data>
)) }""" ] ;
    sh:targetNode <http://shipshape.dyreriket.xyz/std-vocabulary-elements#ANY_NODE> .
